Simu/CommonSem.v
@@ -1,0 +1,55 @@
+Require common.Values.
+
+Require Export Rustre.Common.
+Require Export Rustre.RMemory.
+
+Require Export Syn.
+
+Ltac inv H := inversion H; clear H; subst.
+
+(* SEMANTICS *)
+Definition val: Type := Values.val.
+
+Definition menv: Type := memory val.
+Definition venv: Type := PM.t val.
+
+Definition m_empty: menv := empty_memory _.
+Definition v_empty: venv := PM.empty val.
+
+Definition val_of_const c :=
+  match c with
+  | Cint i => Values.Vint i
+  | Cfloat f => Values.Vfloat f
+  | Csingle s => Values.Vsingle s
+  | Clong l => Values.Vlong l
+  end.
+
+Inductive exp_eval (me: menv) (ve: venv): exp -> val -> Prop :=
+| evar: forall x v ty,
+    PM.MapsTo x v ve ->
+    exp_eval me ve (Var x ty) v
+| estate: forall x v ty,
+    mfind_mem x me = Some v ->
+    exp_eval me ve (State x ty) v
+| econst: forall c ty,
+    exp_eval me ve (Const c ty) (val_of_const c).
+
+Theorem exp_eval_det:
+  forall me ve e v1 v2,
+    exp_eval me ve e v1 ->
+    exp_eval me ve e v2 ->
+    v1 = v2.
+Proof.
+  induction e; intros v1 v2 H1 H2;
+  inversion H1 as [? ? ? Hv1|? ? ? Hv1|];
+  inversion H2 as [? ? ? Hv2|? ? ? Hv2|];
+  auto; unfold PM.MapsTo in *; rewrite Hv1 in Hv2; now injection Hv2.
+Qed.
+
+Ltac app_exp_eval_det :=
+  match goal with
+  | H1: exp_eval ?me ?ve ?e ?v1,
+        H2: exp_eval ?me ?ve ?e ?v2 |- _ =>
+    assert (v1 = v2) by (eapply exp_eval_det; eauto); subst v2; clear H2 
+  end.
+
