Simu/Cor2.v
@@ -1,19 +1,9 @@
-Require cfrontend.Clight.
-Require Import lib.Integers.
-
-Require Import Rustre.Common.
-Require Import Rustre.RMemory.
-
-Require Import Syn Sem2 Tra.
-
-Require Import Program.Tactics.
-Require Import List.
-Import List.ListNotations.
-Open Scope list_scope.
+Require Import CommonCor.
+Require Import Sem2.
 
 (* SIMULATION *)
 
-Section PRESERVATION.
+Section SIMU.
 
   Variable main_node : ident.
   Variable prog: program.
@@ -28,422 +18,38 @@ Section PRESERVATION.
   (* Hypothesis WF: well_formed prog. *)
   Hypothesis MAINNODE: find_class main_node prog = Some (c_main, cls_main).
 
-  (* Lemma well_formed_main: well_formed_cls c_main. *)
-  (* Proof. *)
-  (*   unfold well_formed in WF. *)
-  (*   rewrite Forall_forall in WF. *)
-  (*   apply find_class_In in MAINNODE; auto. *)
-  (* Qed. *)
-    
-  (* Hypothesis BUILD_CO_OK: *)
-  (*   Ctypes.build_composite_env (map translate_class prog.(p_cls)) = Errors.OK (Clight.genv_cenv tge). *)
-
-  (* Hypothesis VE_IN_VARS: forall x v (ve: venv), PM.MapsTo x v ve -> exists t, In (x, t) prog.(p_vars). *)
-
-  Lemma build_co_ok:
-    Ctypes.build_composite_env (map translate_class prog) = Errors.OK (Clight.genv_cenv tge).
-  Proof.
-    unfold translate in TRANSL.
-    rewrite MAINNODE in TRANSL.
-    unfold Clight.make_program in TRANSL.
-    destruct prog.
-    - discriminate.
-    - unfold Ctypes.build_composite_env in *; simpl in *.
-      destruct (translate_class c).
-      admit.
-  Qed.
-  
-  Definition chunk_of_typ ty := AST.chunk_of_type (Ctypes.typ_of_type ty).
-  Definition pointer_of_node node := pointer_of (type_of_inst node).
-  
-  Definition main_fun :=
-    Clight.mkfunction Ctypes.type_int32s AST.cc_default []
-                      c_main.(c_vars)
-                          []
-                          (translate_stmt main_node c_main.(c_step)).
-  
-  Lemma type_pres:
-    forall e, Clight.typeof (translate_exp main_node e) = typeof e.
-  Proof.
-    induction e; simpl; try reflexivity.
-    destruct c; simpl; reflexivity.
-  Qed.
-
-  Definition valid_val (v: val) (t: typ): Prop :=
-    Ctypes.access_mode t = Ctypes.By_value (chunk_of_typ t)
-    /\ v <> Values.Vundef
-    /\ Values.Val.has_type v (Ctypes.typ_of_type t).
-
-  Lemma sem_cast_same:
-    forall v t,
-      valid_val v t ->
-      Cop.sem_cast v t t = Some v.
-  Proof.
-    unfold valid_val; intros; destruct_pairs.
-    destruct t, v;
-      (destruct i, s || destruct f || idtac);
-      (discriminates || contradiction || auto).
-  Qed.
-  
-  (* Lemma tr_main_node: *)
-  (*   exists co, *)
-  (*     Maps.PTree.get main_node (Clight.genv_cenv tge) = Some co *)
-  (*     /\ (forall x (me: menv) v, *)
-  (*           mfind_mem x me = Some v -> *)
-  (*           exists delta, *)
-  (*             Ctypes.field_offset (Clight.genv_cenv tge) x (Ctypes.co_members co) = Errors.OK delta). *)
-  (* Proof. *)
-  (*   destruct MAINNODE as [c [? Hcls]]. *)
-  (*   assert (In (translate_class c) (map translate_class prog.(p_cls))) as Hin. *)
-  (*   - clear TRANSL MAINNODE BUILD_CO_OK. *)
-  (*     apply in_map. *)
-  (*     induction (p_cls prog); simpl in *. *)
-  (*     + discriminate. *)
-  (*     + destruct (ident_eqb (c_name a) main_node). *)
-  (*       * inv Hcls; now left. *)
-  (*       * right; now apply IHl. *)
-  (*   - unfold translate_class in Hin. *)
-  (*     apply find_class_name in Hcls. *)
-  (*     destruct c; simpl in Hcls; subst. *)
-  (*     pose proof (Ctypes.build_composite_env_charact _ _ _ _ _ _ BUILD_CO_OK Hin) as [co Hco]. *)
-  (*     exists co; split. *)
-  (*     * tauto. *)
-  (*     * intros ** Hx. *)
-  (*       admit.                (* how to get a delta witness ??? *) *)
-  (* Qed. *)
-  
-  (* Axiom wt_state_pred: ident * typ -> program -> Prop. *)
-  (* Inductive well_typed_exp: exp -> Prop := *)
-  (* | wt_var: forall x ty, *)
-  (*     In (x, ty) prog.(p_vars) -> *)
-  (*     well_typed_exp (Var x ty) *)
-  (* | wt_state: forall x ty, *)
-  (*     wt_state_pred (x, ty) prog -> *)
-  (*     well_typed_exp (State x ty) *)
-  (* | wt_const: forall c ty, *)
-  (*     well_typed_exp (Const c ty). *)
-
-  (* Inductive well_typed: stmt -> Prop := *)
-  (* | wt_assign: forall x e, *)
-  (*     x <> self_id -> *)
-  (*     In (x, typeof e) prog.(p_vars) -> *)
-  (*     well_typed_exp e -> *)
-  (*     well_typed (Assign x e) *)
-  (* | wt_stassign: forall x e, *)
-  (*     x <> self_id -> *)
-  (*     wt_state_pred (x, typeof e) prog -> *)
-  (*     well_typed_exp e -> *)
-  (*     well_typed (AssignSt x e) *)
-  (* | wt_skip:  *)
-  (*     well_typed Skip. *)
-
-  Definition compat_venv (ve: venv) (env: Clight.env) (m: Memory.Mem.mem):  Prop :=
-    forall x v t,
-      PM.MapsTo x v ve ->
-      In (x, t) c_main.(c_vars) ->
-      exists loc,
-        Maps.PTree.get x env = Some (loc, t)
-        /\ Memory.Mem.load (chunk_of_typ t) m loc 0 = Some v
-        /\ valid_val v t.
-
-  Definition compat_menv (me: menv) (env: Clight.env) (m: Memory.Mem.mem):  Prop :=
-    forall x v t,
-      mfind_mem x me = Some v ->
-      In (x, t) c_main.(c_mems) ->
-      exists co loc' loc ofs delta,
-        Ctypes.field_offset (Clight.genv_cenv tge) x (Ctypes.co_members co) = Errors.OK delta
-        (* /\ In (x, t) (Ctypes.co_members co) *)
-        /\ Memory.Mem.load (chunk_of_typ t) m loc (Int.unsigned (Int.add ofs (Int.repr delta))) = Some v
-        /\ valid_val v t
-        /\ Maps.PTree.get main_node (Clight.genv_cenv tge) = Some co 
-        /\ Maps.PTree.get self_id env = Some (loc', pointer_of_node main_node)
-        /\ Memory.Mem.load (chunk_of_typ (pointer_of_node main_node)) m loc' 0 = Some (Values.Vptr loc ofs)
-        /\ Ctypes.access_mode (pointer_of_node main_node) = Ctypes.By_value (chunk_of_typ (pointer_of_node main_node)).
-
-  Remark valid_val_implies_access:
-    forall v t, valid_val v t -> Ctypes.access_mode t = Ctypes.By_value (chunk_of_typ t).
-  Proof. intros ** H; apply H. Qed.
-    
-  Hint Constructors Clight.eval_lvalue Clight.eval_expr well_formed_stmt(* well_typed *).
-  Hint Resolve valid_val_implies_access.
-  
-  Lemma expr_eval_simu:
-    forall me ve exp v e le m,
-      compat_venv ve e m ->
-      compat_menv me e m ->
-      well_formed_exp c_main exp ->
-      exp_eval me ve exp v ->
-      Clight.eval_expr tge e le m (translate_exp main_node exp) v.
-  Proof.
-    intros me ve exp;
-    induction exp as [x ty|x ty|c ty];
-    intros ** Hvenv Hmenv Hwf Heval;
-    inv Heval; inv Hwf; simpl.
-
-    (* Var x ty : "x" *)
-    - edestruct Hvenv; destruct_conjs; eauto.
-      eapply Clight.eval_Elvalue, Clight.deref_loc_value; eauto.
-
-    (* State x ty : "self->x" *)
-    - edestruct Hmenv; destruct_conjs; eauto.
-      eapply Clight.eval_Elvalue.
-      + eapply Clight.eval_Efield_struct
-        with (id:=main_node) (att:=Ctypes.noattr); eauto.
-        eapply Clight.eval_Elvalue. 
-        * apply Clight.eval_Ederef. 
-          eapply Clight.eval_Elvalue, Clight.deref_loc_value; eauto.
-        * apply Clight.deref_loc_copy; auto.
-      + eapply Clight.deref_loc_value; eauto.
-
-    (* Const c ty : "c" *)
-    - destruct c; constructor.
-  Qed.
-  
-  Definition compat_vars (env: Clight.env): Prop :=
-    forall x t,
-      In (x, t) c_main.(c_vars) ->
-      exists loc, Maps.PTree.get x env = Some (loc, t).
-
-  Definition compat_fields (env: Clight.env) (m: Memory.Mem.mem): Prop :=
-    forall x t,
-      In (x, t) c_main.(c_mems) ->
-      exists co loc' loc ofs delta,
-        Ctypes.field_offset (Clight.genv_cenv tge) x (Ctypes.co_members co) = Errors.OK delta
-        /\ In (x, t) (Ctypes.co_members co)
-        /\ Maps.PTree.get main_node (Clight.genv_cenv tge) = Some co
-        /\ Maps.PTree.get self_id env = Some (loc', pointer_of_node main_node)
-        /\ Memory.Mem.load (chunk_of_typ (pointer_of_node main_node)) m loc' 0 = Some (Values.Vptr loc ofs).
-
-  Definition nodup_env (e: Clight.env) :=
-    forall x x' loc t t',
-      x' <> x ->
-      Maps.PTree.get x e = Some (loc, t) ->
-      Maps.PTree.get x' e <> Some (loc, t').
-
-  Definition nodup_fields (co: Ctypes.composite) :=
-    forall x t t',
-      In (x, t) (Ctypes.co_members co) ->
-      In (x, t') (Ctypes.co_members co) ->
-      t' = t.
-
-  Definition nodup_vars :=
-    forall x t t',
-      In (x, t) c_main.(c_vars) ->
-      In (x, t') c_main.(c_vars) ->
-      t' = t.
-
-   Definition nodup_mems :=
-    forall x t t',
-      In (x, t) c_main.(c_mems) ->
-      In (x, t') c_main.(c_mems) ->
-      t' = t.
-  
-  Inductive compat_stmt: menv -> venv -> Clight.env -> Memory.Mem.mem -> stmt -> Prop :=
-  | compat_assign: forall me ve m (env: Clight.env) e v x loc,
-      exp_eval me ve e v ->
-      Maps.PTree.get x env = Some (loc, typeof e) ->
-      Memory.Mem.valid_access m (chunk_of_typ (typeof e)) loc 0 Memtype.Writable ->
-      valid_val v (typeof e) ->
-      v = Values.Val.load_result (chunk_of_typ (typeof e)) v ->
-      compat_stmt me ve env m (Assign x e)
-  | compat_stassign: forall me ve m (env: Clight.env) e v x co loc' loc ofs delta,
-      exp_eval me ve e v ->
-      Ctypes.field_offset (Clight.genv_cenv tge) x (Ctypes.co_members co) = Errors.OK delta ->
-      In (x, typeof e) (Ctypes.co_members co) ->
-      Maps.PTree.get main_node (Clight.genv_cenv tge) = Some co ->
-      Maps.PTree.get self_id env = Some (loc', pointer_of_node main_node) ->
-      Memory.Mem.load (chunk_of_typ (pointer_of_node main_node)) m loc' 0 = Some (Values.Vptr loc ofs) ->
-                                                                                     
-      Memory.Mem.valid_access m (chunk_of_typ (typeof e)) loc (Int.unsigned (Int.add ofs (Int.repr delta))) Memtype.Writable ->
-      valid_val v (typeof e) ->
-      v = Values.Val.load_result (chunk_of_typ (typeof e)) v ->
-      compat_stmt me ve env m (AssignSt x e)
-  | compat_comp: forall me1 ve1 (* me2 ve2 *) m1 (* m2 *) env s1 s2,
-      compat_stmt me1 ve1 env m1 s1 ->
-      (* stmt_eval (me1, ve1, s1) (me2, ve2, Skip) -> *)
-      (* compat_venv ve2 env m2 -> *)
-      (* compat_menv me2 env m2 -> *)
-      (* compat_stmt me2 ve2 env m2 s2 -> *)
-      compat_stmt me1 ve1 env m1 (Comp s1 s2)
-  | compat_skip: forall me ve m env,
-      compat_stmt me ve env m Skip.
-  
-  Remark find_add:
-    forall x (v v': val) pm, 
-      PM.find x (PM.add x v pm) = Some v' -> v' = v.
-  Proof.
-    induction x, pm; simpl; (eauto || now injection 1).
-  Qed.
-
-  Remark mto_add:
-    forall x v v' (ve: venv),
-      PM.MapsTo x v' (PM.add x v ve) -> v' = v.
-  Proof.
-    unfold PM.MapsTo.
-    apply find_add.
-  Qed.
-
-  Remark mfindmem_add:
-    forall x v v' (me: menv),
-      mfind_mem x (madd_mem x v me) = Some v' -> v' = v.
-  Proof.
-    unfold mfind_mem, madd_mem. simpl.
-    intros; eapply find_add; eauto.
-  Qed.
-  
-  Lemma compat_assign_pres:
-    forall ve me env m loc x e v,
-      compat_venv ve env m ->
-      compat_menv me env m ->
-      nodup_env env ->
-      nodup_vars ->
-      Maps.PTree.get x env = Some (loc, typeof e) ->
-      well_formed_stmt c_main (Assign x e) ->
-      compat_stmt me ve env m (Assign x e) ->
-      exp_eval me ve e v ->
-      exists m', Memory.Mem.store (chunk_of_typ (typeof e)) m loc 0 v = Some m' 
-            /\ compat_venv (PM.add x v ve) env m'
-            /\ compat_menv me env m'.
-  Proof.
-    intros ** Hvenv Hmenv Hnodupenv Hnodupvars Hget Hwf Hcompat ?.
-    inversion_clear Hcompat as [? ? ? ? ? v' ? loc' ? Hget' ? ? Hloadres| | |]. 
-    inversion_clear Hwf as [? ? Hin| | |].
-    rewrite Hget in Hget'; inversion Hget'; subst loc'.        
-    app_exp_eval_det.
-    edestruct Memory.Mem.valid_access_store with (v:=v) as [m']; eauto. 
-    exists m'; repeat split; auto. 
-    - unfold compat_venv; intros x' v' t' Hmto Hin'.
-      destruct (AST.ident_eq x' x) as [|Hx].
-      + subst x'.
-        apply mto_add in Hmto; subst v'.
-        generalize (Hnodupvars _ _ _ Hin Hin'); intro; subst t'. 
-        exists loc; split; [|split]; auto.
-        rewrite Hloadres; eapply Memory.Mem.load_store_same; eauto.
-      + apply PM.add_3 in Hmto; auto.
-        edestruct Hvenv as [loc' [? [Hload]]]; eauto.
-        exists loc'; split; [|split]; auto. 
-        destruct (Values.eq_block loc' loc).
-        * subst loc'.
-          edestruct Hnodupenv; eauto. 
-        * rewrite <-Hload. 
-          eapply Memory.Mem.load_store_other; eauto.
-    - unfold compat_menv; intros x' v' t' Hmem Hin'.
-      edestruct Hmenv
-        as (co & loc'' & loc' & ofs & delta & ? & Hload & ? & ? & Hself' & Hloadptr & ?); eauto.
-      exists co, loc'', loc', ofs, delta.
-      split; [|split; [|split; [|repeat split]]]; auto.
-      + destruct (Values.eq_block loc' loc).
-        * subst loc'.
-          admit.                (* arf *)
-        * rewrite <-Hload.
-          eapply Memory.Mem.load_store_other; eauto.
-      + destruct (Values.eq_block loc'' loc).
-        * subst loc''.
-          edestruct Hnodupenv with (2:=Hget); eauto.
-        * rewrite <-Hloadptr.
-          eapply Memory.Mem.load_store_other; eauto.
-  Qed.
-
-   Lemma compat_stassign_pres:
-    forall ve me env m x e v co loc loc' ofs delta,
-      compat_venv ve env m ->
-      compat_menv me env m ->
-      nodup_mems ->
-      In (x, (typeof e)) (Ctypes.co_members co) ->
-      Ctypes.field_offset tge.(Clight.genv_cenv) x (Ctypes.co_members co) = Errors.OK delta ->
-      Maps.PTree.get main_node (Clight.genv_cenv tge) = Some co ->
-      Maps.PTree.get self_id env = Some (loc', pointer_of_node main_node) ->
-      Memory.Mem.load (chunk_of_typ (pointer_of_node main_node)) m loc' 0 = Some (Values.Vptr loc ofs) ->
-      well_formed_stmt c_main (AssignSt x e) ->
-      compat_stmt me ve env m (AssignSt x e) ->
-      exp_eval me ve e v ->
-      exists m',
-        Memory.Mem.store (chunk_of_typ (typeof e)) m loc (Int.unsigned (Int.add ofs (Int.repr delta))) v = Some m'
-        /\ compat_venv ve env m'
-        /\ compat_menv (madd_mem x v me) env m'.
-  Proof.
-    intros ** Hvenv Hmenv Hnodupmems Hmembers Hoffset Hmain Hself Hloadptr Hwf Hcompat Heval.
-    inversion_clear Hcompat as [|? ? ? ? ? v' ? co' loc1' loc1 ofs' delta' Heval' Hoffset' Hmembers' Hmain' Hself' Hloadptr' ? ? Hloadres| |]. 
-    inversion_clear Hwf as [|? ? Hin| |].
-    rewrite Hmain in Hmain'; inversion Hmain'; subst co'.
-    rewrite Hself in Hself'; inversion Hself'; subst loc1'.
-    rewrite Hoffset in Hoffset'; inversion Hoffset'; subst delta'.
-    rewrite Hloadptr in Hloadptr'; inversion Hloadptr'; subst loc1 ofs'.
-    app_exp_eval_det.
-    edestruct Memory.Mem.valid_access_store with (v:=v) as [m']; eauto. 
-    exists m'; repeat (split; auto).
-    - unfold compat_venv; intros x' v' t' Hmto Hin'.
-      edestruct Hvenv as (loc'' & Hget & Hload' & ?); eauto.
-      exists loc''; split; [|split]; auto.
-      destruct (Values.eq_block loc'' loc).
-      + subst loc''.
-        admit.
-      + rewrite <-Hload'.
-        eapply Memory.Mem.load_store_other; eauto.
-    - unfold compat_menv; intros x' v' t' Hmem Hin'.
-      destruct (AST.ident_eq x' x).
-      + subst x'.
-        apply mfindmem_add in Hmem; subst v'.
-        generalize (Hnodupmems _ _ _ Hin Hin'); intro; subst t'. 
-        exists co, loc', loc, ofs, delta.
-        split; [|split; [|split; [|split; [|repeat split]]]]; auto.
-        * rewrite Hloadres; eapply Memory.Mem.load_store_same; eauto.
-        *{ destruct (Values.eq_block loc' loc).
-           - subst loc'.
-             admit.
-           - rewrite <-Hloadptr.
-             eapply Memory.Mem.load_store_other; eauto.
-         }
-      + rewrite mfind_mem_gso in Hmem; auto.
-        edestruct Hmenv
-          as (co' & loc1' & loc1 & ofs' & delta' & ? & Hload' & ? & Hmain1 & Hself1 & Hloadptr1 & ?); eauto. 
-        rewrite Hmain in Hmain1; inversion Hmain1; subst co'.
-        rewrite Hself in Hself1; inversion Hself1; subst loc1'.
-        rewrite Hloadptr in Hloadptr1; inversion Hloadptr1; subst loc1 ofs'.
-        exists co, loc', loc, ofs, delta'.
-        split; [|split; [|split; [|split; [|repeat split]]]]; auto.
-        * rewrite <-Hload'. eapply Memory.Mem.load_store_other; eauto. right.
-          admit.
-        *{ destruct (Values.eq_block loc' loc).
-           - subst loc'. admit.
-           - rewrite <-Hloadptr.
-             eapply Memory.Mem.load_store_other; eauto.
-         }
-  Qed.
-
-  Inductive compat_cont: menv -> venv -> Clight.env -> Memory.Mem.mem -> cont -> Clight.cont -> Prop :=
-  | compat_kstop: forall me ve e m,
-      compat_cont me ve e m Kstop Clight.Kstop
-  | compat_kseq: forall me ve e m s k k',
+  Inductive compat_cont: (* menv -> venv -> Clight.env -> Memory.Mem.mem -> *) cont -> Clight.cont -> Prop :=
+  | compat_kstop: (* forall me ve e m, *)
+      compat_cont (* me ve e m*) Kstop Clight.Kstop
+  | compat_kseq: forall (* me ve e m *) s k k',
       well_formed_stmt c_main s ->
-      compat_stmt me ve e m s ->
-      compat_cont me ve e m k k' ->
-      compat_cont me ve e m (Kseq s k) (Clight.Kseq (translate_stmt main_node s) k').
-  
+      (* compat_stmt me ve e m s -> *)
+      compat_cont k k' ->
+      compat_cont (* me ve e m *) (Kseq s k) (Clight.Kseq (translate_stmt main_node s) k').  
+
+   
   Inductive match_states: state * stmt * cont -> Clight.state -> Prop :=
-    intro_state: forall me ve s k k' e le m,
-      compat_venv ve e m ->
-      compat_menv me e m ->
+  | intro_state: forall me ve s k k' e le m,
+      compat_venv c_main ve e m ->
+      compat_menv main_node tprog c_main me e m ->
       well_formed_stmt c_main s ->
-      compat_stmt me ve e m s ->
-      (* state_context (me, ve, s) k e le m -> *)
-      compat_cont me ve e m k k' ->
+      compat_stmt main_node tprog me ve e m s ->
+      compat_cont k k' ->
+      mem_sep main_node c_main e m ->
+      self_sep main_node e m ->
+      fields_sep tprog m ->
       nodup_env e ->
-      nodup_vars ->
-      nodup_mems ->
+      nodup_vars c_main ->
+      nodup_mems c_main ->
       match_states
         ((me, ve), s, k)
-        (Clight.State main_fun (translate_stmt main_node s) k' e le m).
-  
+        (Clight.State (main_fun main_node c_main) (translate_stmt main_node s) k' e le m).
+
+  Hint Constructors Clight.eval_lvalue Clight.eval_expr well_formed_stmt.
   Hint Resolve expr_eval_simu Clight.assign_loc_value sem_cast_same.
-  Hint Constructors compat_stmt compat_cont match_states(* state_context *).
-  Hint Constructors well_formed_stmt.
-        
-  Ltac discriminate' :=
-    match goal with
-    | H: ?x <> ?x |- _ => contradict H; reflexivity
-    end.
-  
+  Hint Constructors compat_stmt well_formed_stmt.
+  Hint Constructors match_states compat_cont.
+          
   Theorem simu:
     forall S1 S2,
       stmt_eval_cont S1 S2 ->
@@ -454,19 +60,17 @@ Section PRESERVATION.
           /\ match_states S2 S2'.
   Proof.
     induction 1;
-    inversion_clear 1 as [? ? ? ? ? ? ? ? Hvenv Hmenv Hwf Hstmt (* Hctxt *) Hcont];
-    inv Hwf; inversion_clear Hstmt; (* inversion Hctxt; *)
-    (* (((subst s1 || subst s2); inv_stmt_eval) || destruct_conjs). *)
-    destruct_conjs.
+    inversion_clear 1 as [? ? ? ? ? ? ? ? Hvenv Hmenv Hwf Hstmt Hcont];
+    inv Hwf; inversion_clear Hstmt; destruct_conjs.
     
     (* Assign x e : "x = e" *)
     - app_exp_eval_det.
       edestruct compat_assign_pres as [m']; eauto; destruct_conjs. 
       do 2 econstructor; split.
-      + eapply Smallstep.plus_one, Clight.step_assign; eauto. 
+      + eapply Smallstep.plus_one, Clight.step_assign; eauto. eapply expr_eval_simu; eauto. 
         rewrite type_pres; auto. 
-      + constructor; auto. admit.
-        
+      + constructor; auto. 
+
     (* AssignSt x e : "self->x = e"*)
     - app_exp_eval_det.
       edestruct compat_stassign_pres as [m']; eauto; destruct_conjs. 
@@ -480,17 +84,18 @@ Section PRESERVATION.
              apply Clight.deref_loc_value with (chunk:=AST.Mint32); eauto.
            - apply Clight.deref_loc_copy; auto.
          }
+        * eapply expr_eval_simu; eauto.
         * rewrite type_pres; auto. 
-      + constructor; auto.  admit.
+      + constructor; auto. 
 
     (* Comp s1 s2 : "s1; s2" *)
     - do 2 econstructor; split.
       + eapply Smallstep.plus_one, Clight.step_seq.
-      + constructor; auto. admit.
+      + constructor; auto. 
      
     (* Skip : "skip" *)
     - inv Hcont.
       do 2 econstructor; split.
       + eapply Smallstep.plus_one, Clight.step_skip_seq.
-      + constructor; auto. 
+      + constructor; auto. admit.
   Qed.
